Add memory chunk `Mbool`
It's a 8-bit quantity that is normalized to 0, 1 or Vundef at load time.

This enables a more precise value analysis of loads from pointers to _Boo,
and the corresponding optimizations of casts to _Bool types.

Not yet generated by the C front-end, but correctly treated throughout
the back-end.

common/PrintAST.ml
@@ -37,6 +37,7 @@ let name_of_rettype = function
   | Tint16unsigned -> "int16u"
 
 let name_of_chunk = function
+  | Mbool -> "bool"
   | Mint8signed -> "int8s"
   | Mint8unsigned -> "int8u"
   | Mint16signed -> "int16s"
