common/AST.v
@@ -159,6 +159,7 @@ Definition signature_main :=
   chunk of memory being accessed. *)
 
 Inductive memory_chunk : Type :=
+  | Mbool           (**r 8-bit integer containing 0 or 1 *)
   | Mint8signed     (**r 8-bit signed integer *)
   | Mint8unsigned   (**r 8-bit unsigned integer *)
   | Mint16signed    (**r 16-bit signed integer *)
@@ -180,6 +181,7 @@ Definition Mptr : memory_chunk := if Archi.ptr64 then Mint64 else Mint32.
 
 Definition type_of_chunk (c: memory_chunk) : typ :=
   match c with
+  | Mbool => Tint
   | Mint8signed => Tint
   | Mint8unsigned => Tint
   | Mint16signed => Tint
@@ -199,6 +201,7 @@ Proof. unfold Mptr, Tptr; destruct Archi.ptr64; auto. Qed.
 
 Definition rettype_of_chunk (c: memory_chunk) : rettype :=
   match c with
+  | Mbool => Tint8unsigned
   | Mint8signed => Tint8signed
   | Mint8unsigned => Tint8unsigned
   | Mint16signed => Tint16signed
