x86/Machregs.v
@@ -149,7 +149,7 @@ Definition destroyed_by_load (chunk: memory_chunk) (addr: addressing): list mreg
 
 Definition destroyed_by_store (chunk: memory_chunk) (addr: addressing): list mreg :=
   match chunk with
-  | Mint8signed | Mint8unsigned => if Archi.ptr64 then nil else AX :: CX :: nil
+  | Mbool | Mint8signed | Mint8unsigned => if Archi.ptr64 then nil else AX :: CX :: nil
   | _ => nil
   end.
 
